Work on lab_to_targetProof
With Yong Kiam. Work in progress: trying to figure out the shape of the
Install case of lab_to_targetProof, and the state_rel requirements.

compiler/backend/lab_to_targetScript.sml
@@ -288,7 +288,7 @@ val compile_lab_def = Define `
     if ffis_ok then
       case remove_labels c.init_clock c.asm_conf c.pos c.labels ffis sec_list of
       | SOME (sec_list,l1) =>
-          SOME (prog_to_bytes sec_list,ffis,
+          SOME (prog_to_bytes sec_list,
                 c with <| labels := l1;
                           pos := FOLDL (λpos sec. sec_length (Section_lines sec) pos) c.pos sec_list;
                           ffi_names := SOME ffis
